theories/FOL/Reductions/PCPb_to_ZFD.v
@@ -19,34 +19,6 @@ Local Notation "x / y" := (x, y).
 
 
 
-(** ** Rudimentary tactics for ND manipulations *)
-
-(* Ltac subsimpl_in' H :=
-  rewrite !subst_term_comp, !subst_term_id in H; try now intros [|[|[|[|[|]]]]].
-
-Ltac subsimpl' :=
-  rewrite !subst_term_comp, !subst_term_id; try now intros [|[|[|[|[|]]]]]. *)
-
-Ltac subsimpl_in H :=
-  rewrite ?up_term, ?subst_term_shift in H.
-
-Ltac subsimpl :=
-  rewrite ?up_term, ?subst_term_shift.
-
-Ltac assert1 H :=
-  match goal with |- (?phi :: ?T) ⊢ _ => assert (H : (phi :: T) ⊢ phi) by auto end.
-
-Ltac assert2 H :=
-  match goal with |- (?phi :: ?psi :: ?T) ⊢ _ => assert (H : (phi :: psi :: T) ⊢ psi) by auto end.
-
-Ltac prv_all x :=
-  apply AllI; edestruct nameless_equiv_all as [x ->]; cbn; subsimpl.
-
-Ltac use_exists H x :=
-  apply (ExE _ H); edestruct nameless_equiv_ex as [x ->]; cbn -[comb_rel is_rep]; subsimpl.
-
-
-
 (** ** Simple derivations in ZF *)
 
 Section ZF.
@@ -571,40 +543,42 @@ Proof.
       * apply ZF_eq_prep. auto. eapply opair_inj2; eauto.
 Qed.
 
+Local Arguments comb_rel : simpl never.
+
 Lemma is_rep_eq T B s t x y :
   ZFeq' <<= T -> T ⊢ x ≡ enc_stack B -> T ⊢ is_rep (comb_rel s t) x y
   -> T ⊢ y ≡ enc_stack (append_all B (s / t)).
 Proof.
   intros HT H1 H2. apply ZF_ext'; trivial.
   - prv_all a.
-    apply (AllE a) in H2. cbn -[comb_rel] in H2. subsimpl_in H2.
+    apply (AllE a) in H2. cbn in H2. subsimpl_in H2.
     eapply CE1 in H2. rewrite imps in *.
     use_exists H2 z. assert1 H. apply CE in H as [H H'].
-    unfold comb_rel at 2 in H'. cbn -[comb_rel] in H'. subsimpl_in H'.
-    rewrite !prep_string_subst in H'. cbn -[comb_rel] in H'. 
+    unfold comb_rel at 2 in H'. cbn in H'. subsimpl_in H'.
+    rewrite !prep_string_subst in H'. cbn in H'. 
     use_exists H' c. clear H'.
-    cbn -[comb_rel]. subsimpl. rewrite !prep_string_subst. cbn -[comb_rel].
+    cbn. subsimpl. rewrite !prep_string_subst. cbn.
     assert1 H'. use_exists H' d. clear H'.
-    cbn -[comb_rel]. subsimpl. rewrite !prep_string_subst. cbn -[comb_rel]. subsimpl.
+    cbn. subsimpl. rewrite !prep_string_subst. cbn. subsimpl.
     eapply ZF_eq_elem. auto. apply ZF_sym'. auto.
     eapply CE2. auto. apply ZF_refl'. auto.
     apply append_all_el. auto.
     eapply ZF_eq_elem. auto. eapply CE1. auto.
     eapply (Weak H1). auto. eapply (Weak H). auto.
-  - prv_all a. apply (AllE a) in H2. cbn -[comb_rel] in H2. subsimpl_in H2.
+  - prv_all a. apply (AllE a) in H2. cbn in H2. subsimpl_in H2.
     eapply CE2 in H2. apply II. eapply IE; try apply (Weak H2). auto.
-    induction B as [|[u v] B IH] in T, x, HT, H1 |- *; cbn -[comb_rel] in *.
+    induction B as [|[u v] B IH] in T, x, HT, H1 |- *; cbn in *.
     + apply Exp. eapply IE. apply ZF_eset'. all: auto.
     + rewrite <- imps. apply bunion_use; trivial.
       * specialize (IH T (enc_stack B) HT).
         assert (H : T ⊢ enc_stack B ≡ enc_stack B) by now apply ZF_refl'.
         apply IH in H. use_exists H z. clear H. apply ExI with z.
-        cbn -[comb_rel]. subsimpl. assert1 H. apply CE in H as [H H'].
+        cbn. subsimpl. assert1 H. apply CE in H as [H H'].
         apply CI; trivial. eapply ZF_eq_elem. auto.
         apply ZF_refl'. auto. apply ZF_sym'. auto.
         apply (Weak H1). auto. apply ZF_bunion_el1; trivial. auto.
       * apply ExI with (opair (enc_string u) (enc_string v)).
-        cbn -[comb_rel]. subsimpl. apply CI.
+        cbn. subsimpl. apply CI.
         -- eapply ZF_eq_elem. auto. apply ZF_refl'. auto.
            apply ZF_sym'. auto. apply (Weak H1). auto.
            apply ZF_bunion_el2. auto. eapply Weak. apply ZF_sing_el. auto.
@@ -614,12 +588,14 @@ Proof.
            subsimpl. apply CI; auto. apply ZF_refl'. auto.
 Qed.
 
+Local Arguments is_rep : simpl never.
+
 Lemma combinations_eq T B C x y :
   ZFeq' <<= T -> T ⊢ x ≡ enc_stack C -> T ⊢ combinations B x y -> T ⊢ y ≡ enc_stack (derivation_step B C).
 Proof.
   induction B as [|[s t] B IH] in y, T |-*; cbn; intros HT H1 H2; trivial.
   use_exists H2 u. assert1 H. use_exists H v. clear H.
-  rewrite !combinations_subst, !is_rep_subst. cbn -[is_rep]. subsimpl.
+  rewrite !combinations_subst, !is_rep_subst. cbn. subsimpl.
   eapply ZF_trans'. auto. eapply CE1. eapply CE1. auto.
   eapply ZF_trans'. auto. 2: apply enc_stack_app; auto.
   apply ZF_eq_bunion; auto.
