theories/FOL/Util/FullDeduction.v
@@ -91,6 +91,12 @@ Section ND_def.
     - apply (CE2 H).
   Qed.
 
+  Lemma DE' A phi :
+    A ⊢ phi ∨ phi -> A ⊢ phi.
+  Proof.
+    intros H. apply (DE H); auto.
+  Qed.
+
   Lemma switch_conj_imp alpha beta phi A :
     A ⊢ alpha ∧ beta --> phi <-> A ⊢ alpha --> beta --> phi.
   Proof.
@@ -119,6 +125,54 @@ Notation "A ⊢C phi" := (@prv _ _ _ class A phi) (at level 55).
 Notation "A ⊢I phi" := (@prv _ _ _ intu A phi) (at level 55).
 Notation "A ⊢M phi" := (@prv _ _ falsity_off intu A phi) (at level 55).
 Notation "T ⊢TI phi" := (@tprv _ _ _ intu T phi) (at level 55).
+
+
+
+(** ** Custom induction principle *)
+
+Lemma prv_ind_full {Σ_funcs : funcs_signature} {Σ_preds : preds_signature} :
+  forall P : peirce -> list (form falsity_on) -> (form falsity_on) -> Prop,
+    (forall (p : peirce) (A : list form) (phi psi : form),
+        (phi :: A) ⊢ psi -> P p (phi :: A) psi -> P p A (phi --> psi)) ->
+    (forall (p : peirce) (A : list form) (phi psi : form),
+        A ⊢ phi --> psi -> P p A (phi --> psi) -> A ⊢ phi -> P p A phi -> P p A psi) ->
+    (forall (p : peirce) (A : list form) (phi : form),
+        (map (subst_form ↑) A) ⊢ phi -> P p (map (subst_form ↑) A) phi -> P p A (∀ phi)) ->
+    (forall (p : peirce) (A : list form) (t : term) (phi : form),
+        A ⊢ ∀ phi -> P p A (∀ phi) -> P p A phi[t..]) ->
+    (forall (p : peirce) (A : list form) (t : term) (phi : form),
+        A ⊢ phi[t..] -> P p A phi[t..] -> P p A (∃ phi)) ->
+    (forall (p : peirce) (A : list form) (phi psi : form),
+        A ⊢ ∃ phi ->
+              P p A (∃ phi) ->
+              (phi :: [p[↑] | p ∈ A]) ⊢ psi[↑] -> P p (phi :: [p[↑] | p ∈ A]) psi[↑] -> P p A psi) ->
+    (forall (p : peirce) (A : list form) (phi : form), A ⊢ ⊥ -> P p A ⊥ -> P p A phi) ->
+    (forall (p : peirce) (A : list form) (phi : form), phi el A -> P p A phi) ->
+    (forall (p : peirce) (A : list form) (phi psi : form),
+        A ⊢ phi -> P p A phi -> A ⊢ psi -> P p A psi -> P p A (phi ∧ psi)) ->
+    (forall (p : peirce) (A : list form) (phi psi : form),
+        A ⊢ phi ∧ psi -> P p A (phi ∧ psi) -> P p A phi) ->
+    (forall (p : peirce) (A : list form) (phi psi : form),
+        A ⊢ phi ∧ psi -> P p A (phi ∧ psi) -> P p A psi) ->
+    (forall (p : peirce) (A : list form) (phi psi : form),
+        A ⊢ phi -> P p A phi -> P p A (phi ∨ psi)) ->
+    (forall (p : peirce) (A : list form) (phi psi : form),
+        A ⊢ psi -> P p A psi -> P p A (phi ∨ psi)) ->
+    (forall (p : peirce) (A : list form) (phi psi theta : form),
+        A ⊢ phi ∨ psi ->
+        P p A (phi ∨ psi) ->
+        (phi :: A) ⊢ theta ->
+        P p (phi :: A) theta -> (psi :: A) ⊢ theta -> P p (psi :: A) theta -> P p A theta) ->
+    (forall (A : list form) (phi psi : form), P class A (((phi --> psi) --> phi) --> phi)) ->
+    forall (p : peirce) (l : list form) (f14 : form), l ⊢ f14 -> P p l f14.
+Proof.
+  intros. specialize (prv_ind (fun ff => match ff with falsity_on => P | _ => fun _ _ _ => True end)). intros H'.
+  apply H' with (ff := falsity_on); clear H'. all: intros; try destruct ff; trivial. all: intuition eauto 2.
+Qed.
+
+
+
+(** ** Soundness *)
 
 Section Soundness.
 
@@ -168,3 +222,33 @@ Section Soundness.
   Qed.
 
 End Soundness.
+
+
+
+(** ** Rudimentary tactics for ND manipulations *)
+
+Ltac subsimpl_in H :=
+  rewrite ?up_term, ?subst_term_shift in H.
+
+Ltac subsimpl :=
+  rewrite ?up_term, ?subst_term_shift.
+
+Ltac assert1 H :=
+  match goal with |- (?phi :: ?T) ⊢ _ => assert (H : (phi :: T) ⊢ phi) by auto end.
+
+Ltac assert2 H :=
+  match goal with |- (?phi :: ?psi :: ?T) ⊢ _ => assert (H : (phi :: psi :: T) ⊢ psi) by auto end.
+
+Ltac assert3 H :=
+  match goal with |- (?phi :: ?psi :: ?theta :: ?T) ⊢ _ => assert (H : (phi :: psi :: theta :: T) ⊢ theta) by auto end.
+
+Ltac assert4 H :=
+  match goal with |- (?f :: ?phi :: ?psi :: ?theta :: ?T) ⊢ _ => assert (H : (f :: phi :: psi :: theta :: T) ⊢ theta) by auto end.
+
+Ltac prv_all x :=
+  apply AllI; edestruct nameless_equiv_all as [x ->]; cbn; subsimpl.
+
+Ltac use_exists H x :=
+  apply (ExE _ H); edestruct nameless_equiv_ex as [x ->]; cbn; subsimpl.
+
+
